SATsolver/Experiment/DPLL/misc.lean
@@ -60,3 +60,27 @@ theorem sublist_without_mem {e : α}{l : List α} :
         case tail imem =>
           have := hall.2 i imem neq
           simp[this]
+
+def isEven (n : Nat) : Prop :=
+  ∃ k, k * 2 = n
+
+theorem doubleIseven{n : Nat} : isEven (n*2) := by simp[isEven]
+
+def someFunction (n : Nat)(_ : isEven n) := 4
+
+def callingSomeFunction (n : Nat) :=
+  have doubleEven : isEven (n * 2) := by exact doubleIseven
+  someFunction (n * 2) doubleEven
+
+def returnFithElementOrThree (l : List Nat) :=
+  if longer_than_five : l.length > 5 then l[5]'longer_than_five
+  else 3
+
+
+def subtract (n m : Nat)(_ : n > m) : Nat :=
+  n - m
+
+def sum : List Nat → Nat
+  | [] => 0
+  | n :: ns => n + sum ns
+termination_by x => List.length x
